\documentclass[11pt]{article}
\usepackage{fullpage}
\usepackage{algorithm}
\usepackage[noend]{algorithmic}
\usepackage{amsmath,amssymb,amsthm}
\usepackage{stackrel}

% These define new environments / formats for lemmas, definitions, running time, etc.
\newtheorem{lemma}{Lemma}
\newtheorem{definition}{Definition}
\newtheorem{notation}{Notation}
\newtheorem*{claim}{Claim}
\newtheorem{observation}{Observation}
\newtheorem{conjecture}[lemma]{Conjecture}
\newtheorem{theorem}[lemma]{Theorem}
\newtheorem{corollary}[lemma]{Corollary}
\newtheorem{proposition}[lemma]{Proposition}
\newtheorem*{rt}{Running Time}

% These define nice ways to format P and OPT (use \P or \opt)
\def\P{\ensuremath{$ \mathcal{P} $}}
\def\opt{\ensuremath{\textsc{opt}}}
\renewcommand{\labelenumi}{\bf \alph{enumi}.}
\newcommand{\Z}{\mathbb{Z}}
\newcommand{\linesep}{\noindent\bigskip\rule{17cm}{0.1mm}\bigskip}

\renewcommand\maketitle{
	\begin{center}
		\begin{tabular*}{6.44in}{l @{\extracolsep{\fill}}c r}
			\bfseries  &  & \bfseries CSCI 383 Spring 2019 \\
			\bfseries&  & \bfseries  Homework \#1 Solutions  \\
			\bfseries   &   &  \bfseries Kai Ting Keshia Yap\\ 
		\end{tabular*}
\end{center} }

\begin{document}
	\maketitle
	
	\noindent Honor Code: I affirm that I adhered to the Honor Code in this assignment. Keshia Yap\\
	
	\subsection*{Part 3: Strings}
	We define the reverse of a string recursively as follows: 
	\[\epsilon^R:=\epsilon\]
	\[(wa)^R:=a(w^R)\]
	for all $ a\in \Sigma $ and $ w\in\Sigma^* $. Use this definition and structural induction to prove the following:
	
	\begin{theorem}
		For all $ u,v\in\Sigma^*, (uv)^R=v^Ru^R $.
	\end{theorem}
	\linesep
	
	\begin{proof}
		We proceed by structual induction:\\
		
		Base case: 
%		When $ v=u=\varepsilon $, $ (uv)^R=(\varepsilon\varepsilon)^R=\varepsilon^R=\varepsilon^R\varepsilon=\varepsilon^R\varepsilon^R=v^Ru^R $.\\
		When $ v=\varepsilon $, $ (uv)^R=(u\varepsilon )^R=u^R=\varepsilon u^R=\varepsilon^R u^R =v^R u^R$. \\
%		When $ u=\varepsilon $, $ (uva)^R=(\varepsilon va)^R=(va)^R=av^R av^R\varepsilon=a u^R \varepsilon^R =av^R u^R$.\\		
		
		Inductive hypothesis: Suppose that for some strings $ x,y \in\Sigma^*, (xy)^R=y^Rx^R $.\\
		
		Inductive case: Given $ a\in\Sigma $, by associativity of string concatenation, and since since $ xy \in\Sigma^*$, \[(x(ya))^R=((xy)a)^R=a(xy)^R=ay^Rx^R=(ya)^Rx^R.\]
		\bigskip
		
		Therefore, for all $ u,v\in\Sigma^*, (uv)^R=v^Ru^R $.
	\end{proof}
	
	
\end{document}
